**解：**

 (I) $|\boldsymbol{A}-\lambda \boldsymbol{E}|=\left|\begin{array}{ccc}2-\lambda & -1 & -1 \\\\\\ -1 & 2-\lambda & -1 \\\\\\ -1 & -1 & 2-\lambda\end{array}\right|=-\lambda(3-\lambda)^2=0, \boldsymbol{A}$ 的特征值为 $\lambda_1=0, \lambda_2=\lambda_3=3$.

当 $\lambda_1=0$ 时, 有 $\boldsymbol{A}-0 \boldsymbol{E}=\boldsymbol{A} \sim\left(\begin{array}{ccc}1 & 0 & -1 \\ 0 & 1 & -1 \\ 0 & 0 & 0\end{array}\right)$, 特征向量 $\boldsymbol{\xi}_1=\left(\begin{array}{l}1 \\ 1 \\ 1\end{array}\right)$, 单位化 $\boldsymbol{e}_1=\frac{1}{\sqrt{3}}\left(\begin{array}{l}1 \\ 1 \\ 1\end{array}\right)$;

当 $\lambda_2=3$ 时,有 $\boldsymbol{A}-3 \boldsymbol{E} \sim\left(\begin{array}{lll}1 & 1 & 1 \\\\\\ 0 & 0 & 0 \\\\\\ 0 & 0 & 0\end{array}\right)$, 特征向量 $\boldsymbol{\xi}_2=\left(\begin{array}{c}-1 \\\\\\ 1 \\\\\\ 0\end{array}\right), \boldsymbol{\xi}_3=\left(\begin{array}{c}-1 \\\\\\ 0 \\\\\\ 1\end{array}\right)$, 正交单位化为 $\boldsymbol{e}_2=\frac{1}{\sqrt{2}}\left(\begin{array}{c}-1 \\\\\\ 1 \\\\\\ 0\end{array}\right)$, $\boldsymbol{e}_3=\frac{1}{\sqrt{6}}\left(\begin{array}{c}1 \\\\\\ 1 \\\\\\ -2\end{array}\right)$, 所以 $\boldsymbol{Q}=\left(\begin{array}{ccc}\frac{1}{\sqrt{3}} & \frac{-1}{\sqrt{2}} & \frac{1}{\sqrt{6}} \\\\\\ \frac{1}{\sqrt{3}} & \frac{1}{\sqrt{2}} & \frac{1}{\sqrt{6}} \\\\\\ \frac{1}{\sqrt{3}} & 0 & \frac{-2}{\sqrt{6}}\end{array}\right)$.


<!-- （II) 令 $\boldsymbol{X}=\left(\boldsymbol{x}_1, \boldsymbol{x}_2\right)$, 则 $\boldsymbol{X}^{\mathrm{T}} \boldsymbol{A} \boldsymbol{X}=\left(\boldsymbol{x}_1, \boldsymbol{x}_2\right)^{\mathrm{T}} \boldsymbol{A}\left(\boldsymbol{x}_1, \boldsymbol{x}_2\right)=\left(\begin{array}{ll}\boldsymbol{x}_1^{\mathrm{T}} \boldsymbol{A} \boldsymbol{x}_1 & \boldsymbol{x}_1^{\mathrm{T}} \boldsymbol{A} \boldsymbol{x}_2 \\\\\\ \boldsymbol{x}_2^{\mathrm{T}} \boldsymbol{A} \boldsymbol{x}_1 & \boldsymbol{x}_2^{\mathrm{T}} \boldsymbol{A} \boldsymbol{x}_2\end{array}\right)=\left(\begin{array}{ll}0 & 0 \\\\\\ 0 & 0\end{array}\right) \cdot \boldsymbol{x}_1^{\mathrm{T}} \boldsymbol{A} \boldsymbol{x}_1=0$, 因为 $\boldsymbol{Q}^{\mathrm{T}} \boldsymbol{A} \boldsymbol{Q}=\boldsymbol{\Lambda}$, 即 $\boldsymbol{A}=\boldsymbol{Q} \boldsymbol{\Lambda} \boldsymbol{Q}^{\mathrm{T}}$, 代人 $\boldsymbol{x}_1^{\mathrm{T}} \boldsymbol{A} \boldsymbol{x}_1=0$, 得
$$
\left(\boldsymbol{Q}^{\mathrm{T}} \boldsymbol{x}_1\right)^{\mathrm{T}} \boldsymbol{\Lambda}\left(\boldsymbol{Q}^{\mathrm{T}} \boldsymbol{x}_1\right)=0 .
$$

令 $\boldsymbol{y}=\boldsymbol{Q}^{\mathrm{T}} \boldsymbol{x}_1$, 即 $\boldsymbol{y}^{\mathrm{T}} \boldsymbol{\Lambda} \boldsymbol{y}=0$, 若 $\boldsymbol{y}=\left(\begin{array}{l}y_1 \\\\\\ y_2 \\\\\\ y_3\end{array}\right)$, 有 $0 \cdot y_1^2+3 y_2^2+3 y_3^2=0$, 故
$$
\boldsymbol{y}=\left(\begin{array}{c}
k_1 \\\\\\
0 \\\\\\
0
\end{array}\right), \quad k_1 \in \mathbb{R}
$$

从而 $\boldsymbol{x}_1=\boldsymbol{Q} \boldsymbol{y}=\frac{k_1}{\sqrt{3}}\left(\begin{array}{l}1 \\\\\\ 1 \\\\\\ 1\end{array}\right) \triangleq\left(\begin{array}{l}k_1 \\\\\\ k_1 \\\\\\ k_1\end{array}\right), k_1 \in \mathbb{R}$.
类似的, 由 $\boldsymbol{x}_2^{\mathrm{T}} \boldsymbol{A} \boldsymbol{x}_2=0$, 可求得 $\boldsymbol{x}_2=\boldsymbol{Q} \boldsymbol{y}=\frac{k_2}{\sqrt{3}}\left(\begin{array}{l}1 \\\\\\ 1 \\\\\\ 1\end{array}\right) \triangleq\left(\begin{array}{l}k_2 \\\\\\ k_2 \\\\\\ k_2\end{array}\right), k_2 \in \mathbb{R}$.
由上可知, $\boldsymbol{x}_2=k \boldsymbol{x}_1$, 所以
$$
\boldsymbol{x}_1^{\mathrm{T}} \boldsymbol{A} \boldsymbol{x}_2=\boldsymbol{x}_2^{\mathrm{T}} \boldsymbol{A} \boldsymbol{x}_1=k \boldsymbol{x}_1^{\mathrm{T}} \boldsymbol{A} \boldsymbol{x}_1=0,
$$

故对任意的 $k_1, k_2, \boldsymbol{X}=\left(\boldsymbol{x}_1, \boldsymbol{x}_2\right)=\left(\begin{array}{ll}k_1 & k_2 \\\\\\ k_1 & k_2 \\\\\\ k_1 & k_2\end{array}\right), k_1, k_2 \in \mathbb{R}$, 满足 $\boldsymbol{X}^{\mathrm{T}} \boldsymbol{A X}=\boldsymbol{O}$.
当 $k_1=k_2=0$ 时, $r(\boldsymbol{X})=0$, 当 $k_1, k_2$ 不全为 0 时, $r(\boldsymbol{X})=1$. -->